Engine/PikeTree.v
@@ -1,6 +1,6 @@
 (** * Pike Tree Algorithm  *)
 
-(* An algorithm that takes a tree as input, and finds the first match *)
+(* An algorithm that takes a tree as input, and finds the first or all matches *)
 (* Its execution is close to the kind of execution the PikeVM is doing on the bytecode *)
 (* It explores multiples ordered branches in parallel, synced with their current input position *)
 (* It also records in a "seen" set, *)
@@ -12,7 +12,7 @@ Import ListNotations.
 From Stdlib Require Import Lia.
 
 From Linden Require Import Regex Chars Groups Tree.
-From Linden Require Import PikeSubset SeenSets.
+From Linden Require Import PikeSubset SeenSets PikeVM.
 From Linden Require Import Parameters BooleanSemantics Semantics.
 From Warblre Require Import Base RegExpRecord.
 
@@ -80,8 +80,8 @@ Section PikeTree.
 
   (* The semantic states of the PikeTree algorithm *)
   Inductive pike_tree_state : Type :=
-  | PTS (inp:input) (active: list (tree * group_map)) (best: option leaf) (blocked: list (tree * group_map)) (future: option tree) (seen:seentrees)
-  | PTS_final (best: option leaf).
+  | PTS (inp:input) (active: list (tree * group_map)) (occ: occurrence) (blocked: list (tree * group_map)) (future: option tree) (seen:seentrees)
+  | PTS_final (occ: occurrence).
 
   (* when generating a new active tree at the beginning, or when doing the acceleration step,
      we may erase the new `future` as long as it does not contain a result.
@@ -108,9 +108,9 @@ Section PikeTree.
     "there exists an initial state" which is useful, since we care about particular
     initializations of the PikeTree which follow the PikeVM execution *)
   Definition pike_tree_initial_state_unanchored (t:tree) (future:option tree) (i:input) : pike_tree_state :=
-    PTS i [pike_tree_initial_tree t] None [] future initial_seentrees.
+    PTS i [pike_tree_initial_tree t] (Best None) [] future initial_seentrees.
   Definition pike_tree_initial_state (t:tree) (i:input) : pike_tree_state :=
-    PTS i [pike_tree_initial_tree t] None [] None initial_seentrees.
+    PTS i [pike_tree_initial_tree t] (Best None) [] None initial_seentrees.
 
   (* non-deterministic acceleration by skipping head branches with no results *)
   (* `tree_acceleration inp future inp' future' t` means that for future tree at *)
@@ -136,432 +136,64 @@ Section PikeTree.
   | pts_skip:
   (* skip an active tree if it has been seen before *)
   (* this is non-deterministic, we can also not skip it by using the other rules *)
-    forall inp t gm active best blocked future seen
+    forall inp t gm active occ blocked future seen
       (SEEN: inseen seen t = true),
-      pike_tree_step (PTS inp ((t,gm)::active) best blocked future seen) (PTS inp active best blocked future seen)
+      pike_tree_step (PTS inp ((t,gm)::active) occ blocked future seen) (PTS inp active occ blocked future seen)
   | pts_acc:
   (* if there are no more active or blocked trees and we have some future, *)
   (* we accelerate by non-deterministically skipping branches with no results *)
-    forall inp best seen nextinp future acc t next_future
+    forall inp occ seen nextinp future acc t next_future
       (ACC: tree_acceleration inp future nextinp acc t)
       (ERASE: may_erase acc next_future),
-      pike_tree_step (PTS inp [] best [] (Some future) seen) (PTS nextinp [pike_tree_initial_tree t] best [] next_future initial_seentrees)
+      pike_tree_step (PTS inp [] occ [] (Some future) seen) (PTS nextinp [pike_tree_initial_tree t] occ [] next_future initial_seentrees)
   | pts_final:
   (* moving to a final state when there are no more active or blocked trees *)
-    forall inp best future seen
-      (LEAF: option_flat_map (fun t => first_leaf t inp) future = None),
-      pike_tree_step (PTS inp [] best [] future seen) (PTS_final best)
+    forall inp occ future seen
+      (LEAF: option_flat_map (fun t => tree_leaves t GroupMap.empty inp forward) future = []),
+      pike_tree_step (PTS inp [] occ [] future seen) (PTS_final occ)
   | pts_nextchar:
     (* when the list of active trees is empty, restart from the blocked ones, proceeding to the next character *)
     (* resetting the seen trees *)
-    forall inp best blocked tgm seen,
-      pike_tree_step (PTS inp [] best (tgm::blocked) None seen) (PTS (next_inp inp) (tgm::blocked) best [] None initial_seentrees)
+    forall inp occ blocked tgm seen,
+      pike_tree_step (PTS inp [] occ (tgm::blocked) None seen) (PTS (next_inp inp) (tgm::blocked) occ [] None initial_seentrees)
   | pts_nextchar_generate:
     (* when the list of active trees is empty and the next tree is a segment of a lazy star prefix, *)
     (* restart from the blocked ones and the head iteration of the lazy star, proceeding to the next character *)
     (* resetting the seen trees *)
-    forall inp c next pref best blocked tgm future t1 t2 seen next_future
+    forall inp c next pref occ blocked tgm future t1 t2 seen next_future
       (INPUT: inp = Input (c::next) pref)
       (FUTURE: future = Some (lazy_iter c t1 t2))
       (ERASE: may_erase t2 next_future),
-      pike_tree_step (PTS inp [] best (tgm::blocked) future seen) (PTS (Input next (c::pref)) ((tgm::blocked) ++ [pike_tree_initial_tree t1]) best [] next_future initial_seentrees)
+      pike_tree_step (PTS inp [] occ (tgm::blocked) future seen) (PTS (Input next (c::pref)) ((tgm::blocked) ++ [pike_tree_initial_tree t1]) occ [] next_future initial_seentrees)
   | pts_nextchar_filter:
     (* when the list of active trees is empty and the next tree is a segment of a lazy star prefix, *)
     (* and the head iteration of the lazy star contains no result, *)
     (* restart from the blocked ones, proceeding to the next character *)
     (* resetting the seen trees *)
-    forall inp c next pref best blocked tgm future t1 t2 seen
+    forall inp c next pref occ blocked tgm future t1 t2 seen
       (INPUT: inp = Input (c::next) pref)
       (FUTURE: future = Some (lazy_iter c t1 t2))
       (LEAF: first_leaf t1 (Input next (c::pref)) = None),
-      pike_tree_step (PTS inp [] best (tgm::blocked) future seen) (PTS (Input next (c::pref)) (tgm::blocked) best [] (Some t2) initial_seentrees)
+      pike_tree_step (PTS inp [] occ (tgm::blocked) future seen) (PTS (Input next (c::pref)) (tgm::blocked) occ [] (Some t2) initial_seentrees)
   | pts_active:
     (* generated new active trees: add them in front of the low-priority ones *)
-    forall inp t gm active best blocked future nextactive seen1 seen2
+    forall inp t gm active occ blocked future nextactive seen1 seen2
       (STEP: tree_bfs_step t gm inp = StepActive nextactive)
       (ADD_SEEN: add_seentrees seen1 t = seen2),
-      pike_tree_step (PTS inp ((t,gm)::active) best blocked future seen1) (PTS inp (nextactive++active) best blocked future seen2)
+      pike_tree_step (PTS inp ((t,gm)::active) occ blocked future seen1) (PTS inp (nextactive++active) occ blocked future seen2)
   | pts_match:
     (* a match is found, discard remaining low-priority active trees *)
-    forall inp t gm active best blocked future seen1 seen2
+    forall inp t gm active active' occ occ' blocked future seen1 seen2
       (STEP: tree_bfs_step t gm inp = StepMatch)
-      (ADD_SEEN: add_seentrees seen1 t = seen2),
-      pike_tree_step (PTS inp ((t,gm)::active) best blocked future seen1) (PTS inp [] (Some (inp,gm)) blocked None seen2)
+      (ADD_SEEN: add_seentrees seen1 t = seen2)
+      (ACC: accept occ inp gm active = (active', occ')),
+      pike_tree_step (PTS inp ((t,gm)::active) occ blocked future seen1) (PTS inp active' occ' blocked None seen2)
   | pts_blocked:
   (* add the new blocked thread after the previous ones *)
-    forall inp t gm active best blocked newt future seen1 seen2
+    forall inp t gm active occ blocked newt future seen1 seen2
       (STEP: tree_bfs_step t gm inp = StepBlocked newt)
       (ADD_SEEN: add_seentrees seen1 t = seen2),
-      pike_tree_step (PTS inp ((t,gm)::active) best blocked future seen1) (PTS inp active best (blocked ++ [(newt,gm)]) future seen2).
-
-  (** * Pike Tree Seen Correction  *)
-
-
-  (** * Non-deterministic tree results *)
-  (* any possible result after skipping or not any sub-tree in the seen set *)
-  Inductive tree_nd: tree -> group_map -> input -> seentrees -> option leaf -> Prop :=
-  | tr_skip:
-    forall seen t gm inp
-      (SEEN: inseen seen t = true),
-      tree_nd t gm inp seen None
-  | tr_mismatch:
-    forall gm inp seen, tree_nd Mismatch gm inp seen None
-  | tr_match:
-    forall gm inp seen, tree_nd Match gm inp seen (Some (inp,gm))
-  | tr_choice:
-    forall t1 t2 gm inp l1 l2 seen
-      (TR1: tree_nd t1 gm inp seen l1)
-      (TR2: tree_nd t2 gm inp seen l2),
-      tree_nd (Choice t1 t2) gm inp seen (seqop l1 l2)
-  | tr_read:
-    forall t cd gm inp l seen
-      (TR: tree_nd t gm (next_inp inp) seen l),
-      tree_nd (Read cd t) gm inp seen l
-  | tr_progress:
-    forall t gm inp l seen
-      (TR: tree_nd t gm inp seen l),
-      tree_nd (Progress t) gm inp seen l
-  | tr_anchorpass:
-    forall a t gm inp l seen
-      (TR: tree_nd t gm inp seen l),
-      tree_nd (AnchorPass a t) gm inp seen l
-  | tr_groupaction:
-    forall t act gm inp l seen
-      (TR: tree_nd t (GroupMap.update (idx inp) act gm) inp seen l),
-      tree_nd (GroupAction act t) gm inp seen l
-  | tr_lookaround:
-    forall lk tlk t gm gm' inp l seen
-      (RES_LK: lk_result lk tlk gm inp = Some gm')
-      (TR: tree_nd t gm' inp seen l),
-      tree_nd (LK lk tlk t) gm inp seen l
-  (* When the tree is constructed by `is_tree`, this case can never happen *)
-  (* since LK tree node is constructed only when `lk_result` returns `Some`. *)
-  (* However, here we operate on arbitrary trees so we must handle this case. *)
-  | tr_lookaroundnone:
-    forall lk tlk t gm inp seen
-      (RES_LK: lk_result lk tlk gm inp = None),
-      tree_nd (LK lk tlk t) gm inp seen None
-  | tr_lookaroundfail:
-    forall lk tlk gm inp seen, tree_nd (LKFail lk tlk) gm inp seen None.
-
-  (* the normal result, obtained with function tree_res without skipping anything, is a possible result *)
-  Lemma tree_res_nd:
-    forall t gm inp seen,
-      pike_subtree t ->
-      tree_nd t gm inp seen (tree_res t gm inp forward).
-  Proof.
-    induction t; intros; simpl; try solve[pike_subset]; try solve[constructor; auto].
-    (* lookarounds *)
-    destruct positivity eqn:Hpos, tree_res eqn:Hres; try destruct l.
-    2, 3: eapply tr_lookaroundnone; unfold lk_result; now rewrite Hpos, Hres.
-    - eapply tr_lookaround.
-      + unfold lk_result. now rewrite Hpos, Hres.
-      + eapply IHt2; pike_subset.
-    - eapply tr_lookaround.
-      + unfold lk_result. now rewrite Hpos, Hres.
-      + eapply IHt2; pike_subset.
-  Qed.
-
-  (* when there is nothing in seen, there is only one possible result *)
-  Lemma tree_nd_initial:
-    forall t gm inp res,
-      pike_subtree t ->
-      tree_nd t gm inp initial_seentrees res ->
-      res = tree_res t gm inp forward.
-  Proof.
-    intros t gm inp res PIKE H.
-    remember initial_seentrees as init.
-    induction H; simpl; pike_subset; auto.
-    - subst. rewrite initial_nothing in SEEN. inversion SEEN.
-    - pike_subset. specialize (IHtree_nd1 H3 eq_refl).
-      specialize (IHtree_nd2 H4 eq_refl). subst. auto.
-    - unfold lk_result in RES_LK.
-      destruct positivity, (tree_res tlk); easy || (try destruct l0; injection RES_LK as <-; eauto).
-    - unfold lk_result in RES_LK.
-      destruct positivity, (tree_res tlk); now try destruct l.
-  Qed.
-
-  (** * List Results  *)
-  (* first possible result in a list of trees - deterministic and non-deterministic versions *)
-
-  Definition list_result (l:list (tree * group_map * input)) : option leaf :=
-    seqop_list l (fun tgmi => tree_res (fst (fst tgmi)) (snd (fst tgmi)) (snd tgmi) forward).
-
-  Lemma list_result_cons:
-    forall t gm l inp,
-      list_result ((t,gm,inp)::l) = seqop (tree_res t gm inp forward) (list_result l).
-  Proof.
-    intros. unfold list_result. destruct (tree_res t gm inp forward) eqn:RES.
-    - erewrite seqop_list_head_some; simpl; eauto.
-    - erewrite seqop_list_head_none; simpl; eauto.
-  Qed.
-
-  Lemma list_result_app:
-    forall l1 l2,
-      list_result (l1 ++ l2) = seqop (list_result l1) (list_result l2).
-  Proof.
-    intros l1. induction l1; intros; auto.
-    destruct a as [[t gm] inp]. unfold list_result.
-    destruct (tree_res t gm inp forward) eqn:RES.
-    - erewrite seqop_list_head_some; simpl; eauto.
-      erewrite seqop_list_head_some; simpl; eauto.
-    - erewrite seqop_list_head_none; simpl; eauto.
-      erewrite seqop_list_head_none; simpl; eauto.
-  Qed.
-
-  Inductive list_nd: list (tree * group_map * input) -> seentrees -> option leaf -> Prop :=
-  | tlr_nil:
-    forall seen, list_nd [] seen None
-  | tlr_cons:
-    forall t gm active inp seen l1 l2 l3
-      (TR: tree_nd t gm inp seen l1)
-      (TLR: list_nd active seen l2)
-      (SEQ: l3 = seqop l1 l2),
-      list_nd ((t,gm,inp)::active) seen l3.
-
-  (* the normal result for a list, without skipping anything, is a possible result *)
-  Lemma list_result_nd:
-    forall active seen,
-      pike_list active ->
-      list_nd active seen (list_result active).
-  Proof.
-    intros active. induction active; try destruct a as [[t gm] i]; intros; pike_subset; try constructor.
-    rewrite list_result_cons.
-    econstructor; eauto. apply tree_res_nd. auto.
-  Qed.
-
-  (* when there is nothing in seen, there is only one possible result *)
-  Lemma list_nd_initial:
-    forall l res,
-      pike_list l ->
-      list_nd l initial_seentrees res ->
-      res = list_result l.
-  Proof.
-    intros l res PIKE H.
-    remember initial_seentrees as init.
-    induction H; simpl; auto; pike_subset.
-    rewrite list_result_cons. specialize (IHlist_nd H1 (eq_refl _)). subst.
-    apply tree_nd_initial in TR; subst; auto.
-  Qed.
-
-  Inductive state_nd: input -> list (tree*group_map) -> option leaf -> list (tree*group_map) -> option tree -> seentrees -> option leaf -> Prop :=
-  | sr:
-    forall blocked active best inp future seen r1 r2 r3 rseq
-      (BLOCKED: list_result (suppl blocked (next_inp inp)) = r1)
-      (ACTIVE: list_nd (suppl active inp) seen r2)
-      (FUTURE: option_flat_map (fun t => first_leaf t inp) future = r3)
-      (SEQ: rseq = seqop r1 (seqop r2 (seqop r3 best))),
-      state_nd inp active best blocked future seen rseq.
-
-  (* Invariant of the PikeTree execution *)
-  (* at any moment, all the possible results of the current state are all equal (equal to the first result of the original tree) *)
-  (* at any moment, all trees manipulated by the algorithms are trees for the subset of regexes supported  *)
-  Inductive piketreeinv: pike_tree_state -> option leaf -> Prop :=
-  | pi:
-    forall result blocked active best inp future seen
-      (SAMERES: forall res, state_nd inp active best blocked future seen res -> res = result)
-      (SUBSET_AC: pike_list (suppl active inp))
-      (SUBSET_BL: pike_list (suppl blocked (next_inp inp)))
-      (SUBSET_NE: match future with | Some t => pike_subtree t | None => True end),
-      piketreeinv (PTS inp active best blocked future seen) result
-  | sr_final:
-    forall best,
-      piketreeinv (PTS_final best) best.
-
-  (** * Non-deterministic results of empty trees  *)
-  Lemma state_nd_future_none:
-    forall inp active best blocked future seen res,
-      first_leaf future inp = None ->
-      state_nd inp active best blocked None seen res ->
-      state_nd inp active best blocked (Some future) seen res.
-  Proof.
-    intros inp active best blocked future seen res ERASE ND.
-    inversion ND; subst. simpl in ND.
-    econstructor; eauto.
-  Qed.
-
-  Theorem state_nd_erase:
-    forall inp active best blocked future seen res erased,
-      may_erase future erased ->
-      state_nd inp active best blocked erased seen res ->
-      state_nd inp active best blocked (Some future) seen res.
-  Proof.
-    intros inp active best blocked future seen res erased ERASE ND.
-    inversion ERASE; subst; auto.
-    eapply state_nd_future_none; eauto using res_indep.
-  Qed.
-
-
-
-  (** * Initialization  *)
-
-  (* In the initial state, the invariant holds *)
-
-  Lemma init_piketree_inv:
-    forall t inp,
-      pike_subtree t ->
-      piketreeinv (pike_tree_initial_state t inp) (first_leaf t inp).
-  Proof.
-    intros t. unfold first_leaf. unfold pike_tree_initial_state. constructor; simpl; pike_subset; auto.
-    intros res STATEND. inversion STATEND; subst.
-    simpl. rewrite seqop_none. inversion ACTIVE; subst.
-    inversion TLR; subst. rewrite seqop_none.
-    apply tree_nd_initial in TR; auto.
-  Qed.
-
-  Lemma init_piketree_inv_unanchored:
-    forall t r inp tree future,
-      pike_regex r ->
-      initial_future_unanchored r inp future ->
-      bool_tree rer [Areg r] inp CanExit forward t ->
-      bool_tree rer [Areg (lazy_prefix r)] inp CanExit forward tree ->
-      piketreeinv (pike_tree_initial_state_unanchored t future inp) (first_leaf tree inp).
-  Proof.
-    unfold initial_future_unanchored, future_tree_shape.
-    intros t r inp tree future PIKEREG [tree' [FUTURESHAPE FUTUREINIT]] T TREE.
-    assert (pike_subtree t). {
-      eapply pike_actions_pike_tree; try eapply bool_to_istree_regex with (gm:=GroupMap.empty); eauto; pike_subset.
-    }
-    destruct FUTUREINIT as [future|].
-    {
-      assert (pike_subtree future). {
-        eapply subset_semantics; eauto; pike_subset.
-      }
-      assert (Heq: tree = Choice t (GroupAction (Reset []) future)). {
-        inversion TREE; inversion CONT; destruct plus; [discriminate|]; subst.
-        apply bool_tree_determ with (t1:=titer) in FUTURESHAPE; auto.
-        apply bool_tree_determ with (t1:=tskip) in T; auto.
-        now subst.
-      }
-      unfold first_leaf. unfold pike_tree_initial_state_unanchored. constructor; simpl; pike_subset; auto.
-      intros res STATEND. inversion STATEND; subst.
-      simpl. rewrite seqop_none. inversion ACTIVE; subst.
-      inversion TLR; subst. rewrite seqop_none.
-      apply tree_nd_initial in TR; auto.
-      unfold initial_future_unanchored in FUTURESHAPE; subst; auto.
-    }
-    {
-      (* if we initialize future to None, this is exactly init_piketree_inv *)
-      assert (Heq: first_leaf tree inp = first_leaf t inp). {
-        inversion TREE. inversion CONT. destruct plus; [discriminate|subst].
-        replace titer with t0 by eauto using bool_tree_determ.
-        replace tskip with t by eauto using bool_tree_determ.
-        unfold first_leaf in *. simpl. apply res_indep with (inp2:=inp) (gm2:=GroupMap.empty) (dir2:=forward) in NORES as ->. now destruct (tree_res t).
-      } rewrite Heq.
-      now eapply init_piketree_inv.
-    }
-  Qed.
-
-  (** * Non deterministic results lemmas  *)
-
-  (* when lk_result returns none, it is independent of the gm and the inp *)
-  Lemma lk_result_indep_none:
-    forall lk tlk gm1 gm2 inp1 inp2,
-      lk_result lk tlk gm1 inp1 = None ->
-      lk_result lk tlk gm2 inp2 = None.
-  Proof.
-    unfold lk_result.
-    intros lk tlk gm1 gm2 inp1 inp2 H.
-    destruct positivity, tree_res eqn:Hres.
-    - now destruct l.
-    - erewrite res_indep; eauto.
-    - now eapply res_indep_some in Hres as [l' ->].
-    - easy.
-  Qed.
-
-  (* when lk_result returns some, it is independent of the gm and the inp *)
-  Lemma lk_result_indep_some:
-    forall lk tlk gm1 gm2 inp1 inp2 res1,
-      lk_result lk tlk gm1 inp1 = Some res1 ->
-      exists res2, lk_result lk tlk gm2 inp2 = Some res2.
-  Proof.
-    unfold lk_result.
-    intros lk tlk gm1 gm2 inp1 inp2 res1 H.
-    destruct positivity, tree_res eqn:Hres; try discriminate.
-    - eapply res_indep_some in Hres as [l' ->].
-      destruct l'. eauto.
-    - erewrite res_indep; eauto.
-  Qed.
-
-  (* a tree_nd having no results is independent of the gm and the inp *)
-  Lemma no_tree_result_nd:
-    forall t seen gm1 gm2 inp1 inp2
-      (NORES: tree_nd t gm1 inp1 seen None),
-      tree_nd t gm2 inp2 seen None.
-  Proof.
-    induction t; intros;
-      try solve[inversion NORES; subst; try solve[constructor; auto]; try solve [constructor; eapply IHt; eauto]].
-    - inversion NORES; subst.
-      + apply tr_skip. auto.
-      + destruct l1, l2; inversion H.
-        apply tr_choice; eauto.
-    - inversion NORES; subst.
-      + apply tr_skip. auto.
-      + eapply lk_result_indep_some in RES_LK as [gm'' RES_LK''].
-        eapply tr_lookaround; eauto.
-      + eapply tr_lookaroundnone.
-        eapply lk_result_indep_none; eauto.
-  Qed.
-
-  (* skipping over a new tree doesn't change the result if the tree that is being skipped does not have results *)
-  Lemma add_seen:
-    forall t seen tseen gm inp res
-      (NORES: tree_res tseen gm inp forward = None)
-      (TREEND: tree_nd t gm inp (add_seentrees seen tseen) res)
-      (SUBSET: pike_subtree tseen),
-      tree_nd t gm inp seen res.
-  Proof.
-    intros t seen tseen gm inp res NORES TREEND SUBSET.
-    remember (add_seentrees seen tseen) as add.
-    induction TREEND; subst; try solve[constructor; auto];
-      try solve [econstructor; eauto; apply IHTREEND; auto; eapply res_indep; eauto].
-    apply in_add in SEEN as [EQ | SEEN].
-    - subst. rewrite <- NORES. apply tree_res_nd; auto.
-    - apply tr_skip. auto.
-  Qed.
-
-  (* same lemma generalizes to lists of trees *)
-  Lemma list_add_seen:
-    forall l seen tseen gm inp res
-      (NORES: tree_res tseen gm inp forward = None)
-      (LISTND: list_nd l (add_seentrees seen tseen) res)
-      (SUBSET: pike_subtree tseen),
-      list_nd l seen res.
-  Proof.
-    intros l seen tseen gm inp res NORES LISTND SUBSET.
-    remember (add_seentrees seen tseen) as add.
-    induction LISTND; subst; econstructor; eauto.
-    eapply add_seen; eauto. eapply res_indep; eauto.
-  Qed.
-
-  (* skipping over a new tree doesn't change the result if the tree that is being skipped can produce a None result *)
-  Lemma add_seen_nd:
-    forall t seen tseen gm inp res
-      (NORES: tree_nd tseen gm inp seen None)
-      (TREEND: tree_nd t gm inp (add_seentrees seen tseen) res),
-      tree_nd t gm inp seen res.
-  Proof.
-    intros t seen tseen gm inp res NORES TREEND.
-    remember (add_seentrees seen tseen) as add.
-    induction TREEND; subst; try solve[constructor; auto];
-      try solve [econstructor; eauto; apply IHTREEND; auto; eapply no_tree_result_nd; eauto].
-    - apply in_add in SEEN as [EQ | SEEN].
-      + subst. apply NORES.
-      + apply tr_skip. auto.
-  Qed.
-
-  (* same lemma generalizes to lists of trees *)
-  Lemma list_add_seen_nd:
-    forall l seen tseen gm inp res
-      (NORES: tree_nd tseen gm inp seen None)
-      (LISTND: list_nd l (add_seentrees seen tseen) res),
-      list_nd l seen res.
-  Proof.
-    intros l seen tseen gm inp res NORES LISTND.
-    remember (add_seentrees seen tseen) as add.
-    induction LISTND; subst; econstructor; eauto.
-    eapply add_seen_nd; eauto. eapply no_tree_result_nd; eauto.
-  Qed.
+      pike_tree_step (PTS inp ((t,gm)::active) occ blocked future seen1) (PTS inp active occ (blocked ++ [(newt,gm)]) future seen2).
 
 
   Lemma tree_acceleration_pike_subtree:
@@ -606,6 +238,262 @@ Section PikeTree.
     lia.
   Qed.
 
+  (** * Pike Tree Seen Correction  *)
+
+
+  (** * Non-deterministic tree results *)
+  (* any possible results after skipping or not any sub-tree in the seen set *)
+  Inductive tree_nd: tree -> group_map -> input -> seentrees -> list leaf -> Prop :=
+  | tr_skip:
+    forall seen t gm inp
+      (SEEN: inseen seen t = true),
+      tree_nd t gm inp seen []
+  | tr_mismatch:
+    forall gm inp seen, tree_nd Mismatch gm inp seen []
+  | tr_match:
+    forall gm inp seen, tree_nd Match gm inp seen [(inp,gm)]
+  | tr_choice:
+    forall t1 t2 gm inp l1 l2 seen
+      (TR1: tree_nd t1 gm inp seen l1)
+      (TR2: tree_nd t2 gm inp seen l2),
+      tree_nd (Choice t1 t2) gm inp seen (l1 ++ l2)
+  | tr_read:
+    forall t cd gm inp l seen
+      (TR: tree_nd t gm (next_inp inp) seen l),
+      tree_nd (Read cd t) gm inp seen l
+  | tr_progress:
+    forall t gm inp l seen
+      (TR: tree_nd t gm inp seen l),
+      tree_nd (Progress t) gm inp seen l
+  | tr_anchorpass:
+    forall a t gm inp l seen
+      (TR: tree_nd t gm inp seen l),
+      tree_nd (AnchorPass a t) gm inp seen l
+  | tr_groupaction:
+    forall t act gm inp l seen
+      (TR: tree_nd t (GroupMap.update (idx inp) act gm) inp seen l),
+      tree_nd (GroupAction act t) gm inp seen l
+  | tr_lookaround:
+    forall lk tlk t gm gm' inp l seen
+      (RES_LK: lk_result lk tlk gm inp = Some gm')
+      (TR: tree_nd t gm' inp seen l),
+      tree_nd (LK lk tlk t) gm inp seen l
+  (* When the tree is constructed by `is_tree`, this case can never happen *)
+  (* since LK tree node is constructed only when `lk_result` returns `Some`. *)
+  (* However, here we operate on arbitrary trees so we must handle this case. *)
+  | tr_lookaroundnone:
+    forall lk tlk t gm inp seen
+      (RES_LK: lk_result lk tlk gm inp = None),
+      tree_nd (LK lk tlk t) gm inp seen []
+  | tr_lookaroundfail:
+    forall lk tlk gm inp seen, tree_nd (LKFail lk tlk) gm inp seen [].
+
+  (* the normal result, obtained with function tree_leaves without skipping anything, is a possible result *)
+  Lemma tree_leaves_nd:
+    forall t gm inp seen,
+      pike_subtree t ->
+      tree_nd t gm inp seen (tree_leaves t gm inp forward).
+  Proof.
+    induction t; intros; simpl; try solve[pike_subset]; try solve[constructor; auto].
+    (* lookarounds *)
+    destruct positivity eqn:Hpos, tree_leaves eqn:Hres; try destruct l.
+    - eapply tr_lookaroundnone. unfold lk_result.
+      rewrite <-first_tree_empty in Hres.
+      now rewrite Hpos, Hres.
+    - eapply first_tree_some in Hres.
+      eapply tr_lookaround.
+      + unfold lk_result. now rewrite Hpos, Hres.
+      + eapply IHt2; pike_subset.
+    - rewrite <-first_tree_empty in Hres.
+      eapply tr_lookaround.
+      + unfold lk_result. now rewrite Hpos, Hres.
+      + eapply IHt2; pike_subset.
+    - eapply tr_lookaroundnone. unfold lk_result.
+      eapply first_tree_some in Hres.
+      now rewrite Hpos, Hres.
+  Qed.
+
+  (* when there is nothing in seen, there is only one possible result *)
+  Lemma tree_nd_initial:
+    forall t gm inp res,
+      pike_subtree t ->
+      tree_nd t gm inp initial_seentrees res ->
+      res = tree_leaves t gm inp forward.
+  Proof.
+    intros t gm inp res PIKE H.
+    remember initial_seentrees as init.
+    induction H; simpl; pike_subset; auto.
+    - subst. rewrite initial_nothing in SEEN. inversion SEEN.
+    - pike_subset. specialize (IHtree_nd1 H3 eq_refl).
+      specialize (IHtree_nd2 H4 eq_refl). subst. auto.
+    - unfold lk_result in RES_LK.
+      destruct positivity, (tree_leaves tlk) eqn:Hleaves; try destruct l0;
+        (rewrite <-first_tree_empty in Hleaves || eapply first_tree_some in Hleaves); rewrite Hleaves in RES_LK;
+        easy || (injection RES_LK as <-; eauto).
+    - unfold lk_result in RES_LK.
+      destruct positivity, (tree_leaves tlk) eqn:Hleaves; try destruct l;
+        (rewrite <-first_tree_empty in Hleaves || eapply first_tree_some in Hleaves); rewrite Hleaves in RES_LK; easy.
+  Qed.
+
+  (** * List Results  *)
+  (* all possible results in a list of trees - deterministic and non-deterministic versions *)
+
+  Definition list_result (l:list (tree * group_map * input)) : list leaf :=
+    flat_map (fun tgmi => tree_leaves (fst (fst tgmi)) (snd (fst tgmi)) (snd tgmi) forward) l.
+
+  Lemma list_result_app:
+    forall l1 l2,
+      list_result (l1 ++ l2) = (list_result l1) ++ (list_result l2).
+  Proof.
+    induction l1; intros; auto; simpl.
+    now rewrite <-app_assoc, IHl1.
+  Qed.
+
+  Inductive list_nd: list (tree * group_map * input) -> seentrees -> list leaf -> Prop :=
+  | tlr_nil:
+    forall seen, list_nd [] seen []
+  | tlr_cons:
+    forall t gm active inp seen l1 l2 l3
+      (TR: tree_nd t gm inp seen l1)
+      (TLR: list_nd active seen l2)
+      (SEQ: l3 = l1 ++ l2),
+      list_nd ((t,gm,inp)::active) seen l3.
+
+  (* the normal result for a list, without skipping anything, is a possible result *)
+  Lemma list_result_nd:
+    forall active seen,
+      pike_list active ->
+      list_nd active seen (list_result active).
+  Proof.
+    intros active. induction active; try destruct a as [[t gm] i]; intros; pike_subset; try constructor.
+    simpl; econstructor; eauto. apply tree_leaves_nd. auto.
+  Qed.
+
+  (* when there is nothing in seen, there is only one possible result *)
+  Lemma list_nd_initial:
+    forall l res,
+      pike_list l ->
+      list_nd l initial_seentrees res ->
+      res = list_result l.
+  Proof.
+    intros l res PIKE H.
+    remember initial_seentrees as init.
+    induction H; simpl; auto; pike_subset.
+    apply tree_nd_initial in TR as <-; eauto.
+    now rewrite IHlist_nd.
+  Qed.
+
+  (** * Non deterministic results lemmas  *)
+
+  (* when lk_result returns none, it is independent of the gm and the inp *)
+  Lemma lk_result_indep_none:
+    forall lk tlk gm1 gm2 inp1 inp2,
+      lk_result lk tlk gm1 inp1 = None ->
+      lk_result lk tlk gm2 inp2 = None.
+  Proof.
+    unfold lk_result.
+    intros lk tlk gm1 gm2 inp1 inp2 H.
+    destruct positivity, tree_res eqn:Hres.
+    - now destruct l.
+    - erewrite res_indep; eauto.
+    - now eapply res_indep_some in Hres as [l' ->].
+    - easy.
+  Qed.
+
+  (* when lk_result returns some, it is independent of the gm and the inp *)
+  Lemma lk_result_indep_some:
+    forall lk tlk gm1 gm2 inp1 inp2 res1,
+      lk_result lk tlk gm1 inp1 = Some res1 ->
+      exists res2, lk_result lk tlk gm2 inp2 = Some res2.
+  Proof.
+    unfold lk_result.
+    intros lk tlk gm1 gm2 inp1 inp2 res1 H.
+    destruct positivity, tree_res eqn:Hres; try discriminate.
+    - eapply res_indep_some in Hres as [l' ->].
+      destruct l'. eauto.
+    - erewrite res_indep; eauto.
+  Qed.
+
+  (* a tree_nd having no results is independent of the gm and the inp *)
+  Lemma no_tree_result_nd:
+    forall t seen gm1 gm2 inp1 inp2
+      (NORES: tree_nd t gm1 inp1 seen []),
+      tree_nd t gm2 inp2 seen [].
+  Proof.
+    induction t; intros;
+      try solve[inversion NORES; subst; try solve[constructor; auto]; try solve [constructor; eapply IHt; eauto]].
+    - inversion NORES; subst.
+      + apply tr_skip. auto.
+      + destruct l1, l2; inversion H.
+        apply tr_choice; eauto.
+    - inversion NORES; subst.
+      + apply tr_skip. auto.
+      + eapply lk_result_indep_some in RES_LK as [gm'' RES_LK''].
+        eapply tr_lookaround; eauto.
+      + eapply tr_lookaroundnone.
+        eapply lk_result_indep_none; eauto.
+  Qed.
+
+  (* skipping over a new tree doesn't change the result if the tree that is being skipped does not have results *)
+  Lemma add_seen:
+    forall t seen tseen gm inp res
+      (NORES: tree_leaves tseen gm inp forward = [])
+      (TREEND: tree_nd t gm inp (add_seentrees seen tseen) res)
+      (SUBSET: pike_subtree tseen),
+      tree_nd t gm inp seen res.
+  Proof.
+    intros t seen tseen gm inp res NORES TREEND SUBSET.
+    remember (add_seentrees seen tseen) as add.
+    induction TREEND; subst; try solve[constructor; auto];
+      try solve [econstructor; eauto; apply IHTREEND; auto; eapply leaves_indep; eauto].
+    apply in_add in SEEN as [EQ | SEEN].
+    - subst. rewrite <- NORES. apply tree_leaves_nd; auto.
+    - apply tr_skip. auto.
+  Qed.
+
+  (* same lemma generalizes to lists of trees *)
+  Lemma list_add_seen:
+    forall l seen tseen gm inp res
+      (NORES: tree_leaves tseen gm inp forward = [])
+      (LISTND: list_nd l (add_seentrees seen tseen) res)
+      (SUBSET: pike_subtree tseen),
+      list_nd l seen res.
+  Proof.
+    intros l seen tseen gm inp res NORES LISTND SUBSET.
+    remember (add_seentrees seen tseen) as add.
+    induction LISTND; subst; econstructor; eauto.
+    eapply add_seen; eauto. eapply leaves_indep; eauto.
+  Qed.
+
+  (* skipping over a new tree doesn't change the result if the tree that is being skipped can produce a None result *)
+  Lemma add_seen_nd:
+    forall t seen tseen gm inp res
+      (NORES: tree_nd tseen gm inp seen [])
+      (TREEND: tree_nd t gm inp (add_seentrees seen tseen) res),
+      tree_nd t gm inp seen res.
+  Proof.
+    intros t seen tseen gm inp res NORES TREEND.
+    remember (add_seentrees seen tseen) as add.
+    induction TREEND; subst; try solve[constructor; auto];
+      try solve [econstructor; eauto; apply IHTREEND; auto; eapply no_tree_result_nd; eauto].
+    - apply in_add in SEEN as [EQ | SEEN].
+      + subst. apply NORES.
+      + apply tr_skip. auto.
+  Qed.
+
+  (* same lemma generalizes to lists of trees *)
+  Lemma list_add_seen_nd:
+    forall l seen tseen gm inp res
+      (NORES: tree_nd tseen gm inp seen [])
+      (LISTND: list_nd l (add_seentrees seen tseen) res),
+      list_nd l seen res.
+  Proof.
+    intros l seen tseen gm inp res NORES LISTND.
+    remember (add_seentrees seen tseen) as add.
+    induction LISTND; subst; econstructor; eauto.
+    eapply add_seen_nd; eauto. eapply no_tree_result_nd; eauto.
+  Qed.
+
   (* using the size of the tree will help us make sure that whenever a tree generates active subtrees, *)
   (* none of these subtrees can contain the parent tree that generated them *)
   Fixpoint size (t:tree) : nat :=
@@ -636,6 +524,170 @@ Section PikeTree.
       + apply IHTREEND2; auto. lia.
   Qed.
 
+  (* extensionality for set-like lists *)
+  Definition list_ext {A} (l1 l2: list A) : Prop :=
+    forall x, In x l1 <-> In x l2.
+
+  Definition occurrences (occ: occurrence) : list leaf :=
+    match occ with
+    | Best (Some best) => [best]
+    | Best None => []
+    | All positions => positions
+    end.
+
+  (* the `occurrence` is compatible with the list of leaves *)
+  Definition occurrence_compat (occ: occurrence) (leaves: list leaf) : Prop :=
+    match occ with
+    (* when tracking only the best position, it must be the head of the list *)
+    | Best best => best = hd_error leaves
+    (* when tracking all positions, they must contain the same elements as the list *)
+    | All positions => list_ext positions leaves
+    end.
+
+  (* whether two occurrences are of the same kind *)
+  Definition same_occurrence_kind (occ1 occ2: occurrence) : Prop :=
+    match occ1, occ2 with
+    | Best _, Best _ => True
+    | All _, All _ => True
+    | _, _ => False
+    end.
+
+  Inductive state_nd: input -> list (tree*group_map) -> occurrence -> list (tree*group_map) -> option tree -> seentrees -> occurrence -> Prop :=
+  | sr:
+    forall blocked active occ inp future seen r1 r2 r3 occseq
+      (BLOCKED: list_result (suppl blocked (next_inp inp)) = r1)
+      (ACTIVE: list_nd (suppl active inp) seen r2)
+      (FUTURE: option_flat_map (fun t => tree_leaves t GroupMap.empty inp forward) future = r3)
+      (SEQ: occurrence_compat occseq (r1 ++ r2 ++ r3 ++ occurrences occ))
+      (SAMEKIND: same_occurrence_kind occ occseq),
+      state_nd inp active occ blocked future seen occseq.
+
+  (* Invariant of the PikeTree execution *)
+  (* at any moment, all the possible results of the current state are all equal (equal to the first result of the original tree) *)
+  (* at any moment, all trees manipulated by the algorithms are trees for the subset of regexes supported  *)
+  Inductive piketreeinv: pike_tree_state -> list leaf -> Prop :=
+  | pi:
+    forall leaves blocked active occ inp future seen
+      (COMPAT: forall occres, state_nd inp active occ blocked future seen occres -> occurrence_compat occres leaves)
+      (SUBSET_AC: pike_list (suppl active inp))
+      (SUBSET_BL: pike_list (suppl blocked (next_inp inp)))
+      (SUBSET_FU: match future with | Some t => pike_subtree t | None => True end),
+      piketreeinv (PTS inp active occ blocked future seen) leaves
+  | sr_final:
+    forall occ leaves,
+      occurrence_compat occ leaves ->
+      piketreeinv (PTS_final occ) leaves.
+
+  (** * Non-deterministic results of empty trees  *)
+  Lemma state_nd_future_none:
+    forall inp active best blocked future seen res,
+      tree_leaves future GroupMap.empty inp forward = [] ->
+      state_nd inp active best blocked None seen res ->
+      state_nd inp active best blocked (Some future) seen res.
+  Proof.
+    intros inp active best blocked future seen res ERASE ND.
+    inversion ND; subst. simpl in ND.
+    econstructor; eauto.
+  Qed.
+
+  Theorem state_nd_erase:
+    forall inp active best blocked future seen res erased,
+      may_erase future erased ->
+      state_nd inp active best blocked erased seen res ->
+      state_nd inp active best blocked (Some future) seen res.
+  Proof.
+    intros inp active best blocked future seen res erased ERASE ND.
+    inversion ERASE; subst; auto.
+    unfold first_leaf in NORES. rewrite first_tree_empty in NORES.
+    eapply state_nd_future_none; eauto using leaves_indep.
+  Qed.
+
+
+  (** * Initialization  *)
+
+  (* In the initial state, the invariant holds *)
+
+  Ltac occ_simpl :=
+    match goal with
+    | SAMEKIND: same_occurrence_kind (Best _) ?occ |- _ =>
+      destruct occ; [clear SAMEKIND|inversion SAMEKIND];
+      match goal with
+      | SEQ: occurrence_compat (Best _) _ |- _ => simpl in SEQ; subst
+      | _ => idtac
+      end
+    | SAMEKIND: same_occurrence_kind (All _) ?occ |- _ =>
+      destruct occ; [inversion SAMEKIND|clear SAMEKIND]
+    | _ => idtac
+    end.
+
+  Ltac inv_state_nd :=
+    match goal with
+    | H: state_nd _ _ _ _ _ _ _ |- _ =>
+      inversion_clear H;
+      occ_simpl;
+      subst; simpl
+    end.
+
+  Lemma init_piketree_inv:
+    forall t inp,
+      pike_subtree t ->
+      piketreeinv (pike_tree_initial_state t inp) (tree_leaves t GroupMap.empty inp forward).
+  Proof.
+    intros t. unfold pike_tree_initial_state. constructor; simpl; pike_subset.
+    intros res STATEND. inv_state_nd.
+    rewrite app_nil_r. inversion ACTIVE; subst.
+    inversion TLR; subst. rewrite app_nil_r.
+    apply tree_nd_initial in TR as <-; auto.
+  Qed.
+
+  Lemma init_piketree_inv_unanchored:
+    forall t r inp tree future,
+      pike_regex r ->
+      initial_future_unanchored r inp future ->
+      bool_tree rer [Areg r] inp CanExit forward t ->
+      bool_tree rer [Areg (lazy_prefix r)] inp CanExit forward tree ->
+      piketreeinv (pike_tree_initial_state_unanchored t future inp) (tree_leaves tree GroupMap.empty inp forward).
+  Proof.
+    unfold initial_future_unanchored, future_tree_shape.
+    intros t r inp tree future PIKEREG [tree' [FUTURESHAPE FUTUREINIT]] T TREE.
+    assert (pike_subtree t). {
+      eapply pike_actions_pike_tree; try eapply bool_to_istree_regex with (gm:=GroupMap.empty); eauto; pike_subset.
+    }
+    destruct FUTUREINIT as [future|].
+    {
+      assert (pike_subtree future). {
+        eapply subset_semantics; eauto; pike_subset.
+      }
+      assert (Heq: tree = Choice t (GroupAction (Reset []) future)). {
+        inversion TREE; inversion CONT; destruct plus; [discriminate|]; subst.
+        apply bool_tree_determ with (t1:=titer) in FUTURESHAPE; auto.
+        apply bool_tree_determ with (t1:=tskip) in T; auto.
+        now subst.
+      }
+      unfold pike_tree_initial_state_unanchored. constructor; simpl; pike_subset; auto.
+      intros res STATEND. inv_state_nd.
+      rewrite app_nil_r. inversion ACTIVE; subst.
+      inversion TLR; subst. rewrite app_nil_r.
+      apply tree_nd_initial in TR as ->; auto.
+    }
+    {
+      unfold first_leaf in NORES.
+      rewrite first_tree_empty in NORES.
+      (* if we initialize future to None, this is exactly init_piketree_inv *)
+      assert (Heq: tree_leaves tree GroupMap.empty inp forward = tree_leaves t GroupMap.empty inp forward). {
+        inversion TREE. inversion CONT. destruct plus; [discriminate|subst].
+        replace titer with t0 by eauto using bool_tree_determ.
+        replace tskip with t by eauto using bool_tree_determ.
+        simpl.
+        apply leaves_indep with (inp2:=inp) (gm2:=GroupMap.empty) (dir2:=forward) in NORES as ->.
+        now rewrite app_nil_r.
+      } rewrite Heq.
+      now eapply init_piketree_inv.
+    }
+  Qed.
+
+  (** * Invariant Preservation  *)
+
   Lemma tree_acceleration_pts_preservation:
     forall inp best future nextinp acc t res seen next_future,
       pike_subtree future ->
@@ -646,22 +698,24 @@ Section PikeTree.
   Proof.
     intros inp best future nextinp acc t res seen next_future SUBSET ACC STATEND ERASE.
     pose proof (tree_acceleration_pike_subtree _ _ _ _ _ ACC SUBSET) as [SUBSET_ACC SUBSET_T].
-    inversion STATEND; subst.
+    inv_state_nd.
     apply list_nd_initial in ACTIVE; simpl; pike_subset.
-    econstructor; try econstructor. subst.
-    unfold list_result, seqop_list.
-    induction ACC; subst; simpl.
-    - unfold first_leaf. simpl. unfold advance_input', advance_input.
-      now rewrite <-seqop_assoc.
-    - replace
-        (first_leaf (lazy_iter c t1 t2) (Input (c :: next) pref))
-        with (first_leaf t2 (Input next (c :: pref))).
+    econstructor; try econstructor || eauto. subst.
+    unfold list_result.
+    induction ACC; subst; simpl; unfold advance_input', advance_input; simpl in *.
+    - now rewrite app_nil_r, app_assoc in SEQ.
+    - unfold first_leaf in LEAF.
+      rewrite first_tree_empty in LEAF.
+      rewrite LEAF.
       apply IHACC; eauto; pike_subset.
-      unfold first_leaf. simpl. unfold advance_input', advance_input.
-      unfold first_leaf in LEAF. rewrite LEAF. reflexivity.
   Qed.
 
-  (** * Invariant Preservation  *)
+  (* we can freely append from the left without affecting the equality of two hd_error *)
+  Lemma hd_error_app_l {A}:
+    forall (l1 l2 l: list A),
+      hd_error l1 = hd_error l2 ->
+      hd_error (l ++ l1) = hd_error (l ++ l2).
+  Proof. now destruct l. Qed.
 
   Theorem pts_preservation:
     forall pts1 pts2 res
@@ -674,202 +728,220 @@ Section PikeTree.
     2: { inversion PSTEP. }
     inversion PSTEP; subst; [| | | | | |destruct t; inversion STEP; subst| |].
     (* skipping *)
-    - constructor; pike_subset; auto. intros res STATEND.
-      apply SAMERES. inversion STATEND; subst.
-      econstructor; eauto. replace r2 with (seqop None r2) by (simpl; auto).
-      eapply tlr_cons; eauto. apply tr_skip. auto.
+    - constructor; pike_subset; auto.
+      intros res STATEND.
+      apply COMPAT. inv_state_nd.
+      econstructor; eauto.
+      eapply tlr_cons with (l1:=[]); eauto. apply tr_skip. auto.
     (* acceleration *)
-    - pose proof (tree_acceleration_pike_subtree _ _ _ _ _ ACC SUBSET_NE) as [SUBSET_ACC SUBSET_T].
+    - pose proof (tree_acceleration_pike_subtree _ _ _ _ _ ACC SUBSET_FU) as [SUBSET_ACC SUBSET_T].
       constructor; pike_subset; auto.
-      2: { destruct next_future; inversion ERASE; subst; simpl; pike_subset. }
-      2: { destruct next_future; inversion ERASE; subst; simpl; pike_subset. }
-      intros res STATEND. apply SAMERES.
+      2, 3: destruct next_future; inversion ERASE; subst; simpl; pike_subset.
+      intros res STATEND. apply COMPAT.
       eapply state_nd_erase in STATEND as ERASEND; eauto.
       inversion ERASE; subst; eapply tree_acceleration_pts_preservation; eauto.
     (* final *)
-    - assert (best = result).
-      { apply SAMERES. econstructor; try econstructor. now rewrite LEAF. }
-      subst. constructor.
+    - constructor.
+      apply COMPAT. econstructor; try econstructor.
+      + rewrite LEAF. destruct occ; simpl.
+        * now destruct best.
+        * easy.
+      + now destruct occ.
     (* nextchar *)
-    - constructor; pike_subset; auto. intros res STATEND. inversion STATEND; subst.
+    - constructor; pike_subset; auto.
+      intros res STATEND. inv_state_nd.
       apply list_nd_initial in ACTIVE; pike_subset.
       simpl. subst.
-      apply SAMERES. econstructor; econstructor.
+      apply COMPAT. econstructor; eauto using tlr_nil.
     (* nextchar_generate *)
     - constructor; pike_subset; auto.
-      2: { destruct next_future; inversion ERASE; subst; simpl; pike_subset. }
-      intros res STATEND. apply SAMERES.
-      inversion STATEND; subst.
+      2, 3: destruct next_future; inversion ERASE; subst; simpl; pike_subset.
+      intros res STATEND. apply COMPAT.
+      inv_state_nd.
       apply list_nd_initial in ACTIVE; pike_subset.
-      2:{ simpl; pike_subset. }
-      2:{ destruct next_future; auto. inversion ERASE; subst; pike_subset. }
-      econstructor; try econstructor. unfold next_inp, advance_input', advance_input.
-      simpl. subst.
-      rewrite suppl_app, list_result_app, <-seqop_assoc.
-      unfold list_result at 2, seqop_list. simpl.
-      inversion ERASE; subst; simpl.
+      2: simpl; pike_subset.
+      econstructor; eauto using tlr_nil. simpl in *. unfold next_inp, advance_input', advance_input.
+      subst.
+      rewrite suppl_app, list_result_app, app_assoc in SEQ.
+      unfold list_result at 2 in SEQ.
+      simpl in SEQ. rewrite app_nil_r in SEQ.
+      inversion ERASE; subst; simpl in SEQ.
       (* we did not erase `future` *)
-      + unfold first_leaf. simpl. unfold advance_input', advance_input.
-        now rewrite <-seqop_assoc.
+      * now repeat rewrite app_assoc in *.
       (* we erased `future` *)
-      + unfold first_leaf in NORES |- *.
-        eapply res_indep in NORES.
-        simpl. unfold advance_input', advance_input. rewrite NORES.
-        now destruct (tree_res t1).
+      * unfold first_leaf in NORES.
+        rewrite first_tree_empty in NORES.
+        eapply leaves_indep in NORES.
+        rewrite NORES.
+        now repeat rewrite app_assoc in *.
     (* nextchar_filter *)
-    - constructor; pike_subset; auto. intros res STATEND. inversion STATEND; subst.
+    - constructor; pike_subset; auto.
+      intros res STATEND. inv_state_nd.
       apply list_nd_initial in ACTIVE; pike_subset.
-      simpl. subst.
-      apply SAMERES.
-      econstructor; try econstructor.
-      unfold first_leaf in *; simpl. unfold next_inp, advance_input', advance_input.
+      subst.
+      apply COMPAT.
+      econstructor; eauto using tlr_nil.
+      unfold first_leaf in LEAF.
+      rewrite first_tree_empty in LEAF.
+      simpl in *. unfold next_inp, advance_input', advance_input.
       now rewrite LEAF.
     (* mismatch *)
-    - simpl. constructor; pike_subset; auto. intros res STATEND. inversion STATEND; subst. apply SAMERES.
+    - simpl. constructor; pike_subset; auto.
+      intros res STATEND. inv_state_nd.
+      apply COMPAT.
       econstructor; eauto. econstructor; eauto.
-      + eapply tr_mismatch.
-      + eapply list_add_seen with (gm:=gm) (inp:=inp) in ACTIVE; eauto.
-      + eauto.
+      * eapply tr_mismatch.
+      * eapply list_add_seen with (gm:=gm) (inp:=inp) in ACTIVE; eauto.
+      * eauto.
     (* choice *)
-    - simpl. constructor; pike_subset; auto. intros res STATEND. inversion STATEND; subst.
+    - simpl. constructor; pike_subset; auto.
+      intros res STATEND. inv_state_nd.
       inversion ACTIVE; subst. inversion TLR; subst.
-      apply SAMERES.
+      apply COMPAT.
       apply add_parent_tree in TR.
       2: { simpl. lia. }
       apply add_parent_tree in TR0.
       2: { simpl. lia. }
-      assert (PARENT: tree_nd (Choice t1 t2) gm inp seen (seqop l1 l0)).
+      assert (PARENT: tree_nd (Choice t1 t2) gm inp seen (l1 ++ l0)).
       { apply tr_choice; auto. }
       (* case analysis: did t contribute to the result? *)
-      destruct (seqop l1 l0) as [leaf|] eqn:CHOICE.
-      + econstructor; eauto. rewrite seqop_assoc.
-        eapply tlr_cons; eauto.
-        * apply list_result_nd. auto.
-        * rewrite CHOICE. simpl. auto.
+      destruct (l1 ++ l0) eqn:CHOICE.
       (* when the tree did not contribute, adding it to seen does not change the results *)
-      + destruct l1; destruct l0; inversion CHOICE.
-        econstructor; eauto.
-        eapply list_add_seen_nd with (gm:=gm) in TLR; eauto.
+      * destruct l1, l0; inversion CHOICE.
+        econstructor; simpl; eauto.
         eapply list_add_seen_nd with (gm:=gm) in TLR0; eauto.
         econstructor; eauto.
+      * destruct occ; occ_simpl.
+        -- rewrite app_assoc with (l:=l1), CHOICE.
+           eapply sr with (r2:=(l :: l2) ++ (list_result (suppl active0 inp))); simpl; eauto using hd_error_app_l.
+           econstructor; eauto using list_result_nd.
+        -- admit.
     (* progress fail *)
     - simpl. constructor; pike_subset; auto.
     (* progress *)
-    - simpl. constructor; pike_subset; auto. intros res STATEND. inversion STATEND; subst.
+    - simpl. constructor; pike_subset; auto.
+      intros res STATEND. inv_state_nd.
       inversion ACTIVE; subst.
-      apply SAMERES.
+      apply COMPAT.
       apply add_parent_tree in TR.
       2: { simpl. lia. }
       assert (PARENT: tree_nd (Progress t) gm inp seen l1).
       { apply tr_progress; auto. }
       (* case analysis: did t contribute to the result? *)
-      destruct l1 as [leaf1|].
-      + econstructor; eauto. simpl.
-        eapply tlr_cons; eauto.
-        apply list_result_nd; auto.
+      destruct l1 as [|leaf1].
       (* when the tree did not contribute, adding it to seen does not change the results *)
-      + econstructor; eauto.
+      * econstructor; simpl; eauto.
         eapply list_add_seen_nd with (gm:=gm) in TLR; eauto.
         econstructor; eauto.
+      * destruct occ; occ_simpl.
+        -- eapply sr with (r2:=(leaf1 :: l1) ++ (list_result (suppl active0 inp))); simpl; eauto using hd_error_app_l.
+           econstructor; eauto using list_result_nd.
+        -- admit.
     (* anchor pass *)
     - constructor; simpl; pike_subset; auto.
-      intros res STATEND. inversion STATEND; subst.
+      intros res STATEND. inv_state_nd.
       inversion ACTIVE; subst.
-      apply SAMERES.
+      apply COMPAT.
       apply add_parent_tree in TR.
       2: { simpl. lia. }
       assert (PARENT: tree_nd (AnchorPass a t) gm inp seen l1).
       { apply tr_anchorpass; auto. }
       (* case analysis: did t contribute to the result? *)
-      destruct l1 as [leaf1|].
-      + econstructor; eauto. simpl.
-        eapply tlr_cons; eauto.
-        apply list_result_nd; auto.
+      destruct l1 as [|leaf1].
       (* when the tree did not contribute, adding it to seen does not change the results *)
-      + econstructor; eauto.
+      * econstructor; simpl; eauto.
         eapply list_add_seen_nd with (gm:=gm) in TLR; eauto.
         econstructor; eauto.
+      * destruct occ; occ_simpl.
+        -- eapply sr with (r2:=(leaf1 :: l1) ++ (list_result (suppl active0 inp))); simpl; eauto using hd_error_app_l.
+           econstructor; eauto using list_result_nd.
+        -- admit.
     (* group action *)
-    - simpl. constructor; pike_subset; auto. intros res STATEND. inversion STATEND; subst.
+    - simpl. constructor; pike_subset; auto.
+      intros res STATEND. inv_state_nd.
       inversion ACTIVE; subst.
-      apply SAMERES.
+      apply COMPAT.
       apply add_parent_tree in TR.
       2: { simpl. lia. }
       assert (PARENT: tree_nd (GroupAction g t) gm inp seen l1).
       { apply tr_groupaction; auto. }
       (* case analysis: did t contribute to the result? *)
-      destruct l1 as [leaf1|].
-      + econstructor; eauto. simpl.
-        eapply tlr_cons; eauto.
-        apply list_result_nd; auto.
+      destruct l1 as [|leaf1].
       (* when the tree did not contribute, adding it to seen does not change the results *)
-      + econstructor; eauto.
+      + econstructor; simpl; eauto.
         eapply list_add_seen_nd with (gm:=gm) in TLR; eauto.
         econstructor; eauto.
+      + destruct occ; occ_simpl.
+        * eapply sr with (r2:=(leaf1 :: l1) ++ (list_result (suppl active0 inp))); simpl; eauto using hd_error_app_l.
+           econstructor; eauto using list_result_nd.
+        * admit.
     (* LK *)
     - constructor; try (destruct lk_result eqn:Hlk; injection H0 as <-); pike_subset; auto.
       (* lk_result succeeded *)
-      + intros res STATEND. inversion STATEND; subst.
-        apply SAMERES.
+      + intros res STATEND. inv_state_nd.
+        apply COMPAT.
         inversion ACTIVE; subst.
         apply add_parent_tree in TR.
         2: { simpl. lia. }
         assert (PARENT: tree_nd (LK lk t1 t2) gm inp seen l1).
         { eapply tr_lookaround; eauto. }
         (* case analysis: did t contribute to the result? *)
-        destruct l1 as [leaf1|].
-        * econstructor; eauto. simpl.
-          eapply tlr_cons; eauto.
-          apply list_result_nd; auto.
+        destruct l1 as [|leaf1].
         (* when the tree did not contribute, adding it to seen does not change the results *)
-        * econstructor; eauto.
+        * econstructor; simpl; eauto.
           eapply list_add_seen_nd with (gm:=gm) in TLR; eauto.
           econstructor; eauto.
+        * destruct occ; occ_simpl.
+          -- eapply sr with (r2:=(leaf1 :: l1) ++ (list_result (suppl active0 inp))); simpl; eauto using hd_error_app_l.
+             econstructor; eauto using list_result_nd.
+          -- admit.
       (* lk_result failed *)
-      + intros res STATEND. inversion STATEND; subst. apply SAMERES.
-        econstructor; eauto. econstructor; eauto.
+      + intros res STATEND. inv_state_nd. apply COMPAT.
+        econstructor; simpl; eauto. econstructor; eauto.
         * eapply tr_lookaroundnone; eauto.
         * eapply list_add_seen with (gm:=gm) (inp:=inp) in ACTIVE; eauto; pike_subset.
           unfold lk_result in Hlk. simpl.
-          destruct positivity, tree_res; now try destruct l.
+          destruct positivity, tree_leaves eqn:Hleaves; try destruct l;
+            (rewrite <-first_tree_empty in Hleaves || eapply first_tree_some in Hleaves); rewrite Hleaves in Hlk; easy.
         * eauto.
     (* LKFail *)
-    - simpl. constructor; pike_subset; auto. intros res STATEND. inversion STATEND; subst. apply SAMERES.
+    - simpl. constructor; pike_subset; auto.
+      intros res STATEND. inv_state_nd. apply COMPAT.
       econstructor; eauto. econstructor; eauto.
       + eapply tr_lookaroundfail.
       + eapply list_add_seen with (gm:=gm) (inp:=inp) in ACTIVE; eauto. pike_subset.
       + eauto.
     (* match *)
-    - destruct t; inversion STEP; try now destruct lk_result; subst. constructor; pike_subset; auto.
-      intros res STATEND. inversion STATEND; subst.
-      inversion ACTIVE; subst. simpl.
-      apply SAMERES. eapply sr with (r2:=Some (inp,gm)); eauto.
-      replace (Some (inp,gm)) with (seqop (Some (inp,gm)) (list_result (suppl active0 inp))) by (simpl; auto).
-      econstructor; auto.
-      + apply tr_match.
-      + apply list_result_nd; auto.
+    - destruct t; inversion STEP; try now destruct lk_result; subst.
+      destruct occ; injection ACC as <- <-.
+      + constructor; pike_subset; auto.
+        intros res STATEND. inv_state_nd.
+        inversion ACTIVE; subst. simpl in *.
+        apply (COMPAT (Best (hd_error (list_result (suppl blocked (next_inp inp)) ++ [(inp, gm)])))).
+        eapply sr with (r2:=(inp,gm) :: list_result (suppl active0 inp)); simpl; eauto using hd_error_app_l.
+        econstructor; eauto using tr_match, list_result_nd.
+      + admit.
     (* blocked *)
     - destruct t; inversion STEP; try now destruct lk_result; subst. constructor; pike_subset; auto.
-      intros res STATEND. inversion STATEND; subst.
-      apply SAMERES.
-      rewrite suppl_app. rewrite list_result_app. simpl. rewrite list_result_cons.
-      replace (list_result []) with (None:option leaf).
-      2: { unfold list_result, seqop_list. simpl. auto. }
-      rewrite seqop_none. rewrite <- seqop_assoc. rewrite seqop_assoc with (o3:=(seqop (option_flat_map (fun t : tree => first_leaf t inp) future) best)).
-      econstructor; eauto.
-      destruct (tree_res newt gm (next_inp inp)) eqn:REST.
-      (* if the blocked tree contained a match, then we don't care about the result of active *)
-      (* we can simply use the result obtained without skipping anything *)
-      + eapply tlr_cons.
-        * apply tree_res_nd. pike_subset.
-        * apply list_result_nd; auto.
-        * simpl. unfold next_inp in REST. rewrite REST. simpl. auto.
-      + eapply tlr_cons.
+      intros res STATEND. inv_state_nd.
+      apply COMPAT.
+      rewrite suppl_app, list_result_app in SEQ. simpl in SEQ.
+      rewrite app_nil_r, <-app_assoc, app_assoc with (n:=(option_flat_map (fun t : tree => tree_leaves t GroupMap.empty inp forward) future ++ occurrences occ)) in SEQ.
+      destruct (tree_leaves newt gm (next_inp inp)) eqn:REST.
+      * econstructor; simpl; eauto.
+        eapply tlr_cons.
         (* if the blocked tree did not contain a match, we prove that the adding it to the seen set *)
         (* does not change the skipping of the following active trees, using list_add_seen *)
-        * apply tree_res_nd. pike_subset.
-        * eapply list_add_seen in ACTIVE; eauto. pike_subset.
-        * simpl. unfold next_inp in REST. rewrite REST. simpl. auto.
-  Qed.
+        -- apply tree_leaves_nd. pike_subset.
+        -- eapply list_add_seen in ACTIVE; simpl; eauto. pike_subset.
+        -- simpl. unfold next_inp in REST. rewrite REST. simpl. auto.
+      (* if the blocked tree contained a match, then we don't care about the result of active *)
+      (* we can simply use the result obtained without skipping anything *)
+      * eapply sr with (r2:=(l :: l0) ++ list_result (suppl active0 inp)); simpl; eauto using hd_error_app_l.
+        eapply tlr_cons.
+        -- apply tree_leaves_nd. pike_subset.
+        -- apply list_result_nd; auto.
+        -- simpl. unfold next_inp in REST. rewrite REST. simpl. auto.
+  Admitted.
 
 End PikeTree.
